@prefix : <http://www.semanticweb.org/ontologies/2025/smart-technical-advisory-ontology/> .
@prefix dbo: <http://dbpedia.org/ontology/> .
@prefix omg: <https://www.omg.org/spec/LCC/Countries/ISO3166-1-CountryCodes/> .
@prefix owl: <http://www.w3.org/2002/07/owl#> .
@prefix rdf: <http://www.w3.org/1999/02/22-rdf-syntax-ns#> .
@prefix xml: <http://www.w3.org/XML/1998/namespace> .
@prefix xsd: <http://www.w3.org/2001/XMLSchema#> .
@prefix rdfs: <http://www.w3.org/2000/01/rdf-schema#> .
@base <http://www.semanticweb.org/ontologies/2025/smart-technical-advisory-ontology/> .

<http://www.semanticweb.org/ontologies/2025/smart-technical-advisory-ontology> rdf:type owl:Ontology ;
                                                                                owl:imports <http://www.ontologydesignpatterns.org/ont/dul/DUL.owl> ,
                                                                                            <http://www.w3.org/ns/org#> ,
                                                                                            <http://xmlns.com/foaf/0.1/> ,
                                                                                            <https://w3id.org/MON/person.owl> ,
                                                                                            <https://www.omg.org/spec/LCC/20211101/Countries/ISO3166-1-CountryCodes/> .

#################################################################
#    Annotation properties
#################################################################

###  http://swrl.stanford.edu/ontologies/3.3/swrla.owl#isRuleEnabled
<http://swrl.stanford.edu/ontologies/3.3/swrla.owl#isRuleEnabled> rdf:type owl:AnnotationProperty .


###  http://xmlns.com/foaf/0.1/member
<http://xmlns.com/foaf/0.1/member> rdf:type owl:AnnotationProperty .


#################################################################
#    Object Properties
#################################################################

###  http://www.semanticweb.org/ontologies/2025/smart-technical-advisory-ontology/aiScenarioType
:aiScenarioType rdf:type owl:ObjectProperty ;
                rdfs:domain :UseCase ;
                rdfs:range :SAPAIScenario ;
                rdfs:comment "It is a property of the use case. It indicates the service request concerns a certain use case that is related to a specific AI Scenario."@en .


###  http://www.semanticweb.org/ontologies/2025/smart-technical-advisory-ontology/belongsToIndustry
:belongsToIndustry rdf:type owl:ObjectProperty ;
                   rdfs:domain :SAPServiceRequest ;
                   rdfs:range :Industry ;
                   rdfs:comment "It is a property of the service request. It indicates the service request belongs to one or more industries (this is because the use case does)."@en .


###  http://www.semanticweb.org/ontologies/2025/smart-technical-advisory-ontology/belongsToSAPProgram
:belongsToSAPProgram rdf:type owl:ObjectProperty ;
                     rdfs:domain :SAPServiceRequest ;
                     rdfs:range :SAPProgramInitiative ;
                     rdfs:comment "It is a property of the service request. It indicates the service request belongs to a SAP program initiative."@en .


###  http://www.semanticweb.org/ontologies/2025/smart-technical-advisory-ontology/belongsToSAPRegion
:belongsToSAPRegion rdf:type owl:ObjectProperty ,
                             owl:FunctionalProperty ;
                    rdfs:domain :Country ;
                    rdfs:range :SAPRegion ;
                    rdfs:comment "It is a property of the country. It indicates the SAP business region the country belongs to."@en .


###  http://www.semanticweb.org/ontologies/2025/smart-technical-advisory-ontology/belongsToServiceRequest
:belongsToServiceRequest rdf:type owl:ObjectProperty ;
                         owl:inverseOf :hasUseCase ;
                         rdfs:domain :UseCase ;
                         rdfs:range :SAPServiceRequest ;
                         rdfs:comment "It indicates the service request the use case is associated to."@en .


###  http://www.semanticweb.org/ontologies/2025/smart-technical-advisory-ontology/btpScenarioType
:btpScenarioType rdf:type owl:ObjectProperty ;
                 rdfs:domain :UseCase ;
                 rdfs:range :SAPBTPScenario ;
                 rdfs:comment "It is a property of the use case. It indicates the use case associated to the service request is related to a specific BTP Scenario."@en .


###  http://www.semanticweb.org/ontologies/2025/smart-technical-advisory-ontology/consistsOf
:consistsOf rdf:type owl:ObjectProperty ;
            rdfs:subPropertyOf owl:topObjectProperty ;
            owl:inverseOf :relatesToServiceRequest ;
            rdfs:domain :SAPServiceRequest ;
            rdfs:range :SAPService ;
            rdfs:comment "It indicates the service requested through the service request."@en .


###  http://www.semanticweb.org/ontologies/2025/smart-technical-advisory-ontology/coversProduct
:coversProduct rdf:type owl:ObjectProperty ;
               rdfs:domain :SAPServiceRequest ;
               rdfs:range :Product ;
               rdfs:comment "It is a property of the service request. It indicates the product involved in the use case that is associated to the service request."@en .


###  http://www.semanticweb.org/ontologies/2025/smart-technical-advisory-ontology/createdBy
:createdBy rdf:type owl:ObjectProperty ,
                    owl:FunctionalProperty ;
           rdfs:domain [ rdf:type owl:Class ;
                         owl:unionOf ( :SAPService
                                       :SAPServiceRequest
                                     )
                       ] ;
           rdfs:range :SAPEmployee ;
           rdfs:comment "It indicates who created the object in the SAP system."@en .


###  http://www.semanticweb.org/ontologies/2025/smart-technical-advisory-ontology/deliveredBy
:deliveredBy rdf:type owl:ObjectProperty ;
             rdfs:subPropertyOf :involves ;
             rdfs:domain :SAPService ;
             rdfs:range :SAPEmployee ;
             rdfs:comment "It indicates who delivered the service to the partner"@en .


###  http://www.semanticweb.org/ontologies/2025/smart-technical-advisory-ontology/executedBy
:executedBy rdf:type owl:ObjectProperty ;
            rdfs:subPropertyOf :involves ;
            rdfs:domain :SAPServiceRequest ;
            rdfs:range :SAPEmployee ;
            rdfs:comment "It indicates who executed the service request"@en .


###  http://www.semanticweb.org/ontologies/2025/smart-technical-advisory-ontology/hasGTMOutcome
:hasGTMOutcome rdf:type owl:ObjectProperty ;
               rdfs:domain :UseCase ;
               rdfs:range :GTMOutcome ;
               rdfs:comment "It is a property of the use case. It indicates the Go-To-Market result the service request produced."@en .


###  http://www.semanticweb.org/ontologies/2025/smart-technical-advisory-ontology/hasGTMRoute
:hasGTMRoute rdf:type owl:ObjectProperty ;
             rdfs:domain :SAPServiceRequest ;
             rdfs:range :GTMRoute ;
             rdfs:comment "It is a property of the service request. It indicates the Go-to-Market result that the service request intends to produce."@en .


###  http://www.semanticweb.org/ontologies/2025/smart-technical-advisory-ontology/hasPartnerContact
:hasPartnerContact rdf:type owl:ObjectProperty ;
                   rdfs:subPropertyOf :involves ;
                   rdfs:domain :SAPServiceRequest ;
                   rdfs:range :SAPPartnerEmployee ;
                   rdfs:comment "It indicates the partner contact person for the service request"@en .


###  http://www.semanticweb.org/ontologies/2025/smart-technical-advisory-ontology/hasPartnerType
:hasPartnerType rdf:type owl:ObjectProperty ;
                rdfs:domain :SAPPartner ;
                rdfs:range :SAPPartnerType ;
                rdfs:comment "It is a property of the partner class. Specifies what type of partner the specific organization is for SAP."@en .


###  http://www.semanticweb.org/ontologies/2025/smart-technical-advisory-ontology/hasPartnershipType
:hasPartnershipType rdf:type owl:ObjectProperty ;
                    rdfs:domain :SAPPartner ;
                    rdfs:range :SAPPartnershipType ;
                    rdfs:comment "It is a property of the partner class. It specifies the type of partnership existing between SAP and a partner."@en .


###  http://www.semanticweb.org/ontologies/2025/smart-technical-advisory-ontology/hasSAPContact
:hasSAPContact rdf:type owl:ObjectProperty ;
               rdfs:domain :SAPServiceType ;
               rdfs:range :SAPEmployee ;
               rdfs:comment "It is a property of the service type class. It indicates the responsible person in SAP (identified by his email address) for the service type offered."@en .


###  http://www.semanticweb.org/ontologies/2025/smart-technical-advisory-ontology/hasUseCase
:hasUseCase rdf:type owl:ObjectProperty ,
                     owl:FunctionalProperty ;
            rdfs:domain :SAPServiceRequest ;
            rdfs:range :UseCase ;
            rdfs:comment "It is a property of the service request class. It indicates the use case associated to the service request."@en .


###  http://www.semanticweb.org/ontologies/2025/smart-technical-advisory-ontology/involvedIn
:involvedIn rdf:type owl:ObjectProperty ;
            rdfs:subPropertyOf owl:topObjectProperty ;
            owl:inverseOf :involves ;
            rdfs:domain <http://xmlns.com/foaf/0.1/Person> ;
            rdfs:range [ rdf:type owl:Class ;
                         owl:unionOf ( :SAPService
                                       :SAPServiceRequest
                                     )
                       ] ;
            rdfs:comment "It indicates the person who is involed in some way in the service request."@en .


###  http://www.semanticweb.org/ontologies/2025/smart-technical-advisory-ontology/involves
:involves rdf:type owl:ObjectProperty ;
          rdfs:domain [ rdf:type owl:Class ;
                        owl:unionOf ( :SAPService
                                      :SAPServiceRequest
                                    )
                      ] ;
          rdfs:range <http://xmlns.com/foaf/0.1/Person> ;
          rdfs:comment "It indicates the service request or service involves a certain person."@en .


###  http://www.semanticweb.org/ontologies/2025/smart-technical-advisory-ontology/isEmployedBy
:isEmployedBy rdf:type owl:ObjectProperty ;
              rdfs:subPropertyOf owl:topObjectProperty ;
              rdf:type owl:FunctionalProperty ;
              rdfs:domain <http://xmlns.com/foaf/0.1/Person> ;
              rdfs:range <http://xmlns.com/foaf/0.1/Organization> ;
              rdfs:comment "It indicates which company the employee is employed by."@en .


###  http://www.semanticweb.org/ontologies/2025/smart-technical-advisory-ontology/modifiedBy
:modifiedBy rdf:type owl:ObjectProperty ;
            rdfs:domain [ rdf:type owl:Class ;
                          owl:unionOf ( :SAPService
                                        :SAPServiceRequest
                                      )
                        ] ;
            rdfs:range :SAPEmployee ;
            rdfs:comment "It indicates who modified the object in the SAP system."@en .


###  http://www.semanticweb.org/ontologies/2025/smart-technical-advisory-ontology/ofCountry
:ofCountry rdf:type owl:ObjectProperty ,
                    owl:FunctionalProperty ;
           rdfs:domain :SAPPartner ;
           rdfs:range :Country ;
           rdfs:comment "It indicates the country of provenance of the SAP partner."@en .


###  http://www.semanticweb.org/ontologies/2025/smart-technical-advisory-ontology/relatesToLoB
:relatesToLoB rdf:type owl:ObjectProperty ;
              rdfs:domain :SAPServiceRequest ;
              rdfs:range :LoB ;
              rdfs:comment "It indicates the line of business the use case associated with the service request refers to."@en .


###  http://www.semanticweb.org/ontologies/2025/smart-technical-advisory-ontology/relatesToServiceRequest
:relatesToServiceRequest rdf:type owl:ObjectProperty ,
                                  owl:FunctionalProperty ;
                         rdfs:domain :SAPService ;
                         rdfs:range :SAPServiceRequest ;
                         rdfs:comment "It is a property of the service class. It indicates the service request the service belongs to."@en .


###  http://www.semanticweb.org/ontologies/2025/smart-technical-advisory-ontology/requested
:requested rdf:type owl:ObjectProperty ;
           rdfs:subPropertyOf owl:topObjectProperty ;
           owl:inverseOf :requestedBy ;
           rdfs:domain :SAPPartner ;
           rdfs:range :SAPServiceRequest ;
           rdfs:comment "It indicates the service request the SAP partner requested."@en .


###  http://www.semanticweb.org/ontologies/2025/smart-technical-advisory-ontology/requestedBy
:requestedBy rdf:type owl:ObjectProperty ;
             rdfs:subPropertyOf owl:topObjectProperty ;
             rdf:type owl:FunctionalProperty ;
             rdfs:domain :SAPServiceRequest ;
             rdfs:range :SAPPartner ;
             rdfs:comment "It is a property of the service request class. It indicates who requested the service request."@en .


###  http://www.semanticweb.org/ontologies/2025/smart-technical-advisory-ontology/requiredSupport
:requiredSupport rdf:type owl:ObjectProperty ;
                 rdfs:domain :SAPServiceRequest ;
                 rdfs:range :RequiredSupport ;
                 rdfs:comment "It is a property of the service request class. It indicates the type of support required in the service request in the context of the associated use case."@en .


###  http://www.semanticweb.org/ontologies/2025/smart-technical-advisory-ontology/responsiblePerson
:responsiblePerson rdf:type owl:ObjectProperty ;
                   rdfs:domain [ rdf:type owl:Class ;
                                 owl:unionOf ( :SAPOrganization
                                               :SAPService
                                             )
                               ] ;
                   rdfs:range :SAPEmployee ;
                   rdfs:comment "Indicates the responsible person in SAP for a certain service or organization."@en .


###  http://www.semanticweb.org/ontologies/2025/smart-technical-advisory-ontology/serviceType
:serviceType rdf:type owl:ObjectProperty ;
             rdfs:domain :SAPService ;
             rdfs:range :SAPServiceType ;
             rdfs:comment "It specifies the type of service requested through a service request."@en .


###  http://www.semanticweb.org/ontologies/2025/smart-technical-advisory-ontology/sourceOfRequest
:sourceOfRequest rdf:type owl:ObjectProperty ,
                          owl:FunctionalProperty ;
                 rdfs:domain :SAPServiceRequest ;
                 rdfs:range :SourceOfRequest ;
                 rdfs:comment """It is a property of the service request class. It indicates which channel the service request originated from. It can be:
'PCD E-Mail'
'PBC request'
'Internal'
'Others'"""@en .


###  http://www.semanticweb.org/ontologies/2025/smart-technical-advisory-ontology/wasInitiatedBy
:wasInitiatedBy rdf:type owl:ObjectProperty ,
                         owl:FunctionalProperty ;
                rdfs:domain :SAPServiceRequest ;
                rdfs:range :SAPServiceRequestInitiator ;
                rdfs:comment """It is a property of the service request class. It indicates who initiated the service request. It can be:
'SAP'
'Customer'
'Partner'"""@en .


#################################################################
#    Data properties
#################################################################

###  http://www.semanticweb.org/ontologies/2025/smart-technical-advisory-ontology/accountName
:accountName rdf:type owl:DatatypeProperty ;
             rdfs:domain :SAPPartner ;
             rdfs:range xsd:string ;
             rdfs:comment "It specifies the account name of the SAP partner."@en .


###  http://www.semanticweb.org/ontologies/2025/smart-technical-advisory-ontology/category
:category rdf:type owl:DatatypeProperty ;
          rdfs:domain [ rdf:type owl:Class ;
                        owl:unionOf ( :Industry
                                      :LoB
                                    )
                      ] ;
          rdfs:range xsd:string ;
          rdfs:comment "It indicates the category of the object it refers to."@en .


###  http://www.semanticweb.org/ontologies/2025/smart-technical-advisory-ontology/completionDate
:completionDate rdf:type owl:DatatypeProperty ;
                rdfs:domain :SAPService ;
                rdfs:range xsd:date ;
                rdfs:comment "It is a property of the service class. It indicates the date of completion of the requested service."@en .


###  http://www.semanticweb.org/ontologies/2025/smart-technical-advisory-ontology/countryCode
:countryCode rdf:type owl:DatatypeProperty ,
                      owl:FunctionalProperty ;
             rdfs:domain :Country ;
             rdfs:range xsd:string ;
             rdfs:comment "It indicates the country code (in the ISO 3166-1 alpha-2 standard) of the country."@en .


###  http://www.semanticweb.org/ontologies/2025/smart-technical-advisory-ontology/createdOnDate
:createdOnDate rdf:type owl:DatatypeProperty ;
               rdfs:domain [ rdf:type owl:Class ;
                             owl:unionOf ( :SAPService
                                           :SAPServiceRequest
                                         )
                           ] ;
               rdfs:range xsd:dateTime ;
               rdfs:comment "It indicates the date the object was created (datetime) in the system."@en .


###  http://www.semanticweb.org/ontologies/2025/smart-technical-advisory-ontology/hasCustomer
:hasCustomer rdf:type owl:DatatypeProperty ;
             rdfs:domain :UseCase ;
             rdfs:range xsd:boolean ;
             rdfs:comment "It marks whether the use case has already a customer or not."@en .


###  http://www.semanticweb.org/ontologies/2025/smart-technical-advisory-ontology/hasDescription
:hasDescription rdf:type owl:DatatypeProperty ;
                rdfs:domain [ rdf:type owl:Class ;
                              owl:unionOf ( :SAPOrganization
                                            :SAPService
                                            :UseCase
                                          )
                            ] ;
                rdfs:range xsd:string ;
                rdfs:comment "This property is used to provide the description of the use case or SAP organization or the service offered by SAP."@en .


###  http://www.semanticweb.org/ontologies/2025/smart-technical-advisory-ontology/hasID
:hasID rdf:type owl:DatatypeProperty ;
       rdfs:domain owl:Thing ;
       rdfs:range xsd:string ;
       rdfs:comment "It indicates the unique identifier of the object in the source table fo the original relational data model."@en .


###  http://www.semanticweb.org/ontologies/2025/smart-technical-advisory-ontology/hasName
:hasName rdf:type owl:DatatypeProperty ;
         rdfs:domain owl:Thing ;
         rdfs:range xsd:string ;
         rdfs:comment "This property indicates the proper name of an object."@en .


###  http://www.semanticweb.org/ontologies/2025/smart-technical-advisory-ontology/hasPBCOrderNumber
:hasPBCOrderNumber rdf:type owl:DatatypeProperty ;
                   rdfs:domain :SAPService ;
                   rdfs:range xsd:string ;
                   rdfs:comment "It indicates the unique  PBC order number of the service (if the service was requested through the Parter Benefits Catalog)."@en .


###  http://www.semanticweb.org/ontologies/2025/smart-technical-advisory-ontology/hasSolution
:hasSolution rdf:type owl:DatatypeProperty ;
             rdfs:domain :SAPServiceRequest ;
             rdfs:range xsd:boolean ;
             rdfs:comment "Flag indicating whether the service request produced a solution."@en .


###  http://www.semanticweb.org/ontologies/2025/smart-technical-advisory-ontology/hasStatus
:hasStatus rdf:type owl:DatatypeProperty ;
           rdfs:domain [ rdf:type owl:Class ;
                         owl:unionOf ( :SAPService
                                       :SAPServiceRequest
                                     )
                       ] ;
           rdfs:range xsd:string ;
           rdfs:comment """It states the status of the service request or of the requested services. It can have the following values:
'requested'/'submitted'
'accepted'
'rejected'
'in progress'
'completed'
'discontinued'
'canceled'"""@en .


###  http://www.semanticweb.org/ontologies/2025/smart-technical-advisory-ontology/hasTitle
:hasTitle rdf:type owl:DatatypeProperty ;
          rdfs:domain :UseCase ;
          rdfs:range xsd:string ;
          rdfs:comment "It indicates the title of the use case associated to the service request."@en .


###  http://www.semanticweb.org/ontologies/2025/smart-technical-advisory-ontology/hasValue
:hasValue rdf:type owl:DatatypeProperty ;
          rdfs:domain owl:Thing ;
          rdfs:range xsd:string ;
          rdfs:comment "This property states the name or type or value assumed by an instance."@en .


###  http://www.semanticweb.org/ontologies/2025/smart-technical-advisory-ontology/isAIUseCase
:isAIUseCase rdf:type owl:DatatypeProperty ;
             rdfs:domain :UseCase ;
             rdfs:range xsd:boolean ;
             rdfs:comment "It marks whether the use case is around AI or not."@en .


###  http://www.semanticweb.org/ontologies/2025/smart-technical-advisory-ontology/isBTPUseCase
:isBTPUseCase rdf:type owl:DatatypeProperty ;
              rdfs:domain :UseCase ;
              rdfs:range xsd:boolean ;
              rdfs:comment "It marks whether the use case involves BTP or not."@en .


###  http://www.semanticweb.org/ontologies/2025/smart-technical-advisory-ontology/isDeleted
:isDeleted rdf:type owl:DatatypeProperty ;
           rdfs:domain :SAPServiceRequest ;
           rdfs:range xsd:boolean ;
           rdfs:comment "Flag that states if the service request is deleted or not."@en .


###  http://www.semanticweb.org/ontologies/2025/smart-technical-advisory-ontology/isFreeService
:isFreeService rdf:type owl:DatatypeProperty ;
               rdfs:domain :SAPService ;
               rdfs:range xsd:boolean ;
               rdfs:comment "It marks whether the requested service is paid or free."@en .


###  http://www.semanticweb.org/ontologies/2025/smart-technical-advisory-ontology/isGSSP
:isGSSP rdf:type owl:DatatypeProperty ;
        rdfs:domain :SAPPartner ;
        rdfs:range xsd:boolean ;
        rdfs:comment "It marks whether an SAP partner is GSSP (global strategic service partner) or not."@en .


###  http://www.semanticweb.org/ontologies/2025/smart-technical-advisory-ontology/legalIPOwner
:legalIPOwner rdf:type owl:DatatypeProperty ;
              rdfs:domain :Product ;
              rdfs:range xsd:string ;
              rdfs:comment "It indicates the legal owner of the intellectual property of a certain product."@en .


###  http://www.semanticweb.org/ontologies/2025/smart-technical-advisory-ontology/modifiedOnDate
:modifiedOnDate rdf:type owl:DatatypeProperty ;
                rdfs:domain [ rdf:type owl:Class ;
                              owl:unionOf ( :SAPService
                                            :SAPServiceRequest
                                          )
                            ] ;
                rdfs:range xsd:dateTime ;
                rdfs:comment "It indicates the date the object was modified (datetime) in the system."@en .


###  http://www.semanticweb.org/ontologies/2025/smart-technical-advisory-ontology/partnerStatus
:partnerStatus rdf:type owl:DatatypeProperty ;
               rdfs:domain :SAPPartner ;
               rdfs:range xsd:string ;
               rdfs:comment """It indicates the status of the SAP partner. It can have the following values:
\"Prospective Partner\"
\"Active\"
\"Discontinued\""""@en .


###  http://www.semanticweb.org/ontologies/2025/smart-technical-advisory-ontology/plannedGoLiveDate
:plannedGoLiveDate rdf:type owl:DatatypeProperty ;
                   rdfs:domain :UseCase ;
                   rdfs:range xsd:date ;
                   rdfs:comment "It indicates the planned go-live date of the solution (if specified) that the service request helped develop."@en .


###  http://www.semanticweb.org/ontologies/2025/smart-technical-advisory-ontology/productName
:productName rdf:type owl:DatatypeProperty ;
             rdfs:domain :Product ;
             rdfs:range xsd:string ;
             rdfs:comment "It indicates the name of the software product."@en .


###  http://www.semanticweb.org/ontologies/2025/smart-technical-advisory-ontology/productPublicName
:productPublicName rdf:type owl:DatatypeProperty ;
                   rdfs:domain :Product ;
                   rdfs:range xsd:string ;
                   rdfs:comment "It indicates the public name of the product."@en .


###  http://www.semanticweb.org/ontologies/2025/smart-technical-advisory-ontology/productType
:productType rdf:type owl:DatatypeProperty ;
             rdfs:domain :Product ;
             rdfs:range xsd:string ;
             rdfs:comment """It indicates the type of the product. It can be:
\"SAP Product\"
\"3rd Party Product\"
\"Service\"
\"Users and Unallocated\""""@en .


###  http://www.semanticweb.org/ontologies/2025/smart-technical-advisory-ontology/requestDate
:requestDate rdf:type owl:DatatypeProperty ;
             rdfs:domain :SAPServiceRequest ;
             rdfs:range xsd:date ;
             rdfs:comment "It is a property of the service request class. It indicates the date the service request was submitted."@en .


###  http://www.semanticweb.org/ontologies/2025/smart-technical-advisory-ontology/revenue
:revenue rdf:type owl:DatatypeProperty ;
         rdfs:domain :SAPService ;
         rdfs:range xsd:float ;
         rdfs:comment "It indicates the revenue earned from the delivery of a certain service."@en .


###  http://www.semanticweb.org/ontologies/2025/smart-technical-advisory-ontology/solutionArea
:solutionArea rdf:type owl:DatatypeProperty ;
              rdfs:domain :Product ;
              rdfs:range xsd:string ;
              rdfs:comment """It indicates the solution area of the product. It can have the following values:
\"HXM\"
\"BPI\"
\"BTP\"
\"S4\"
\"CX\"
\"WCM\"
\"Cross\"
\"XM\"
\"ISBN\""""@en .


###  http://www.semanticweb.org/ontologies/2025/smart-technical-advisory-ontology/solutionSubArea
:solutionSubArea rdf:type owl:DatatypeProperty ;
                 rdfs:subPropertyOf :solutionArea ;
                 rdfs:domain :Product ;
                 rdfs:range xsd:string ;
                 rdfs:comment """It indicates the solution subarea of the product. It can have the following values:
\"Business Network\"
\"Business Process Intelligence\"
\"Commerce\"
\"Core HR and Payroll\"
\"Cross Business Services\"
\"Customer Data Solutions\"
\"Database and Data Management\"
\"Digital Supply Chain\"
\"ERP for SME\"
\"Enterprise Cloud Services (IaaS)\"
\"Experience Management\"
\"External Workforce\"
\"Finance, Q2C and Enterprise Mgmt\"
\"Foundation/Appl. Dev. & Integration\"
\"IBSO Projects\"
\"Industry-specific Applications\"
\"Learning and Talent\"
\"Marketing\"
\"Others\"
\"Planning and Analytics\"
\"Premium Engagements\"
\"Procurement\"
\"Qualtrics EX\"
\"Sales Performance Management\"
\"Sales and Services\"
\"SuccessFactors Cross\"
\"Taulia\"
\"Training and Adoption\"
\"Travel and Expense\""""@en .


###  http://www.semanticweb.org/ontologies/2025/smart-technical-advisory-ontology/startDate
:startDate rdf:type owl:DatatypeProperty ;
           rdfs:domain :SAPService ;
           rdfs:range xsd:date ;
           rdfs:comment "It is a property of the service class. It indicates the date the delivery of the requested service began."@en .


###  http://www.semanticweb.org/ontologies/2025/smart-technical-advisory-ontology/useCaseStatus
:useCaseStatus rdf:type owl:DatatypeProperty ;
               rdfs:domain :UseCase ;
               rdfs:range xsd:string ;
               rdfs:comment """It indicates the status of the use case associated to the partner service request. It can take on one of the following values:
'in progress'
'completed'
'discontinued'
'not yet started'""" .


#################################################################
#    Classes
#################################################################

###  http://www.semanticweb.org/ontologies/2025/smart-technical-advisory-ontology/BTPSolutionArchitect
:BTPSolutionArchitect rdf:type owl:Class ;
                      rdfs:subClassOf :SAPEmployee ;
                      owl:disjointWith :COILExpert ;
                      rdfs:comment "Team of BTP solution architects in SAP who are mandated to coach and guide SAP partners in implementing their solution on BTP."@en .


###  http://www.semanticweb.org/ontologies/2025/smart-technical-advisory-ontology/COILExpert
:COILExpert rdf:type owl:Class ;
            rdfs:subClassOf :SAPEmployee ;
            rdfs:comment "Class of SAP employees that are member of the SAP Co-Innovation Lab, an SAP organization that helps SAP partners to convert ideas for solutions for intelligent enterprises into working prototypes and from there to market-ready solutions."@en .


###  http://www.semanticweb.org/ontologies/2025/smart-technical-advisory-ontology/Country
:Country rdf:type owl:Class ;
         owl:equivalentClass <https://www.omg.org/spec/LCC/Countries/CountryRepresentation/Country> ;
         rdfs:comment "Country where the service is delivered or country of provenance of the partner."@en .


###  http://www.semanticweb.org/ontologies/2025/smart-technical-advisory-ontology/GTMOutcome
:GTMOutcome rdf:type owl:Class ;
            rdfs:comment "Outcome of the Go-to-Market process if there is one related to the service request submitted."@en .


###  http://www.semanticweb.org/ontologies/2025/smart-technical-advisory-ontology/GTMRoute
:GTMRoute rdf:type owl:Class ;
          rdfs:comment "Go-to-Market process expected for the submitted service request."@en .


###  http://www.semanticweb.org/ontologies/2025/smart-technical-advisory-ontology/Industry
:Industry rdf:type owl:Class ;
          rdfs:comment "Industry to which the use case is related to."@en .


###  http://www.semanticweb.org/ontologies/2025/smart-technical-advisory-ontology/LoB
:LoB rdf:type owl:Class ;
     rdfs:comment "Line of businesses the use case is related to."@en .


###  http://www.semanticweb.org/ontologies/2025/smart-technical-advisory-ontology/NamedIndividual
:NamedIndividual rdf:type owl:Class .


###  http://www.semanticweb.org/ontologies/2025/smart-technical-advisory-ontology/Product
:Product rdf:type owl:Class ;
         rdfs:comment "Software product involved in the use case associated to the partner service request."@en .


###  http://www.semanticweb.org/ontologies/2025/smart-technical-advisory-ontology/RequiredSupport
:RequiredSupport rdf:type owl:Class ;
                 rdfs:comment "Type of support required for the service."@en .


###  http://www.semanticweb.org/ontologies/2025/smart-technical-advisory-ontology/SAPAIScenario
:SAPAIScenario rdf:type owl:Class ;
               rdfs:comment """Class of the possible AI scenarios in the SAP domain. It can be:
'Embedded AI'
'BTP AI'
'3rd Party AI'"""@en .


###  http://www.semanticweb.org/ontologies/2025/smart-technical-advisory-ontology/SAPBTPScenario
:SAPBTPScenario rdf:type owl:Class ;
                rdfs:comment """Possible scenario when implementing a solution on SAP BTP. It can be one of the following:
'Data-to-Value'
'Extensibility'
'Integration'"""@en .


###  http://www.semanticweb.org/ontologies/2025/smart-technical-advisory-ontology/SAPEmployee
:SAPEmployee rdf:type owl:Class ;
             owl:equivalentClass [ rdf:type owl:Restriction ;
                                   owl:onProperty <http://xmlns.com/foaf/0.1/member> ;
                                   owl:someValuesFrom :SAPOrganization
                                 ] ;
             rdfs:subClassOf <http://www.ontologydesignpatterns.org/ont/dul/DUL.owl#Person> ,
                             <http://xmlns.com/foaf/0.1/Agent> ,
                             <http://xmlns.com/foaf/0.1/Person> ;
             owl:disjointWith :SAPPartnerEmployee ;
             rdfs:comment "Person who is employed by SAP and that is involved in the coaching services."@en .


###  http://www.semanticweb.org/ontologies/2025/smart-technical-advisory-ontology/SAPOrganization
:SAPOrganization rdf:type owl:Class ;
                 rdfs:subClassOf <http://xmlns.com/foaf/0.1/Organization> ;
                 owl:disjointWith :SAPPartner ;
                 rdfs:comment "Organized group of people in SAP with a particular purpose"@en .


###  http://www.semanticweb.org/ontologies/2025/smart-technical-advisory-ontology/SAPPartner
:SAPPartner rdf:type owl:Class ;
            rdfs:subClassOf <http://xmlns.com/foaf/0.1/Organization> ;
            rdfs:comment "Company that is in a certain business relationship with SAP"@en .


###  http://www.semanticweb.org/ontologies/2025/smart-technical-advisory-ontology/SAPPartnerContact
:SAPPartnerContact rdf:type owl:Class ;
                   rdfs:subClassOf :SAPPartnerEmployee ;
                   rdfs:comment "A partner employee responsible of the service request on the partner side."@en .


###  http://www.semanticweb.org/ontologies/2025/smart-technical-advisory-ontology/SAPPartnerEmployee
:SAPPartnerEmployee rdf:type owl:Class ;
                    owl:equivalentClass [ rdf:type owl:Restriction ;
                                          owl:onProperty :isEmployedBy ;
                                          owl:minQualifiedCardinality "1"^^xsd:nonNegativeInteger ;
                                          owl:onClass :SAPPartner
                                        ] ,
                                        [ rdf:type owl:Restriction ;
                                          owl:onProperty <http://www.w3.org/ns/org#memberOf> ;
                                          owl:minQualifiedCardinality "1"^^xsd:nonNegativeInteger ;
                                          owl:onClass :SAPPartner
                                        ] ;
                    rdfs:subClassOf <http://www.ontologydesignpatterns.org/ont/dul/DUL.owl#Person> ,
                                    <http://xmlns.com/foaf/0.1/Agent> ,
                                    <http://xmlns.com/foaf/0.1/Person> ;
                    rdfs:comment "Person employed by an SAP Partner."@en .


###  http://www.semanticweb.org/ontologies/2025/smart-technical-advisory-ontology/SAPPartnerType
:SAPPartnerType rdf:type owl:Class ;
                rdfs:comment "Type of SAP partner."@en .


###  http://www.semanticweb.org/ontologies/2025/smart-technical-advisory-ontology/SAPPartnershipType
:SAPPartnershipType rdf:type owl:Class ;
                    rdfs:comment "Type of partnership existing between and organization and SAP."@en .


###  http://www.semanticweb.org/ontologies/2025/smart-technical-advisory-ontology/SAPProgramInitiative
:SAPProgramInitiative rdf:type owl:Class ;
                      rdfs:comment "SAP program initiative to which the request is associated."@en .


###  http://www.semanticweb.org/ontologies/2025/smart-technical-advisory-ontology/SAPRegion
:SAPRegion rdf:type owl:Class ;
           rdfs:comment "Class of SAP business regions."@en .


###  http://www.semanticweb.org/ontologies/2025/smart-technical-advisory-ontology/SAPService
:SAPService rdf:type owl:Class ;
            rdfs:comment "Service requested via service request from SAP partner. It is possible that multiple services are associated with the same service request."@en .


###  http://www.semanticweb.org/ontologies/2025/smart-technical-advisory-ontology/SAPServiceRequest
:SAPServiceRequest rdf:type owl:Class ;
                   rdfs:comment "Formal coaching request sent by an SAP partner to SAP. A single request may be used to request multiple services."@en .


###  http://www.semanticweb.org/ontologies/2025/smart-technical-advisory-ontology/SAPServiceRequestInitiator
:SAPServiceRequestInitiator rdf:type owl:Class ;
                            rdfs:comment """Who initiated the service request. It can be:
'SAP'
'Customer'
'Partner'"""@en .


###  http://www.semanticweb.org/ontologies/2025/smart-technical-advisory-ontology/SAPServiceType
:SAPServiceType rdf:type owl:Class ;
                rdfs:comment "Type of service requested to SAP."@en .


###  http://www.semanticweb.org/ontologies/2025/smart-technical-advisory-ontology/SourceOfRequest
:SourceOfRequest rdf:type owl:Class ;
                 rdfs:comment """Channels through which the request can arrive. It can be:
'PCD E-Mail'
'PBC request'
'Internal'
'Others'"""@en .


###  http://www.semanticweb.org/ontologies/2025/smart-technical-advisory-ontology/UseCase
:UseCase rdf:type owl:Class ;
         rdfs:comment "Use case attached to the partner service request."@en .


###  https://www.omg.org/spec/LCC/Countries/CountryRepresentation/Country
<https://www.omg.org/spec/LCC/Countries/CountryRepresentation/Country> rdf:type owl:Class .


#################################################################
#    Individuals
#################################################################

###  http://www.semanticweb.org/ontologies/2025/smart-technical-advisory-ontology#xxxx.yyyyy@sap.com
<http://www.semanticweb.org/ontologies/2025/smart-technical-advisory-ontology#xxxx.yyyyy@sap.com> rdf:type owl:NamedIndividual ,
                                                                                                                  :SAPEmployee ;
                                                                                                         <http://xmlns.com/foaf/0.1/member> :SAPOrg1 ;
                                                                                                         <http://xmlns.com/foaf/0.1/name> "xxxx yyyyy" ;
                                                                                                         <http://xmlns.com/foaf/0.1/mbox> "xxxx.yyyyy@sap.com" .


###  http://www.semanticweb.org/ontologies/2025/smart-technical-advisory-ontology/SAP
:SAP rdf:type owl:NamedIndividual ,
              <http://xmlns.com/foaf/0.1/Organization> ;
     rdfs:comment "SAP SE is a European multinational software company based in Walldorf, Baden-Württemberg, Germany. The company is the world's largest vendor of enterprise resource planning (ERP) software."@en .


###  http://www.semanticweb.org/ontologies/2025/smart-technical-advisory-ontology/SAPOrg1
:SAPOrg1 rdf:type owl:NamedIndividual .


###  http://www.semanticweb.org/ontologies/2025/smart-technical-advisory-ontology/SAPOrg2
:SAPOrg2 rdf:type owl:NamedIndividual .


#################################################################
#    Rules
#################################################################

:x rdf:type <http://www.w3.org/2003/11/swrl#Variable> .

[ <http://swrl.stanford.edu/ontologies/3.3/swrla.owl#isRuleEnabled> "true"^^xsd:boolean ;
   rdfs:comment "" ;
   rdfs:label "S1" ;
   rdf:type <http://www.w3.org/2003/11/swrl#Imp> ;
   <http://www.w3.org/2003/11/swrl#body> [ rdf:type <http://www.w3.org/2003/11/swrl#AtomList> ;
                                           rdf:first [ rdf:type <http://www.w3.org/2003/11/swrl#ClassAtom> ;
                                                       <http://www.w3.org/2003/11/swrl#classPredicate> :SAPEmployee ;
                                                       <http://www.w3.org/2003/11/swrl#argument1> :x
                                                     ] ;
                                           rdf:rest [ rdf:type <http://www.w3.org/2003/11/swrl#AtomList> ;
                                                      rdf:first [ rdf:type <http://www.w3.org/2003/11/swrl#IndividualPropertyAtom> ;
                                                                  <http://www.w3.org/2003/11/swrl#propertyPredicate> <http://xmlns.com/foaf/0.1/member> ;
                                                                  <http://www.w3.org/2003/11/swrl#argument1> :x ;
                                                                  <http://www.w3.org/2003/11/swrl#argument2> :SAPOrg1
                                                                ] ;
                                                      rdf:rest rdf:nil
                                                    ]
                                         ] ;
   <http://www.w3.org/2003/11/swrl#head> [ rdf:type <http://www.w3.org/2003/11/swrl#AtomList> ;
                                           rdf:first [ rdf:type <http://www.w3.org/2003/11/swrl#ClassAtom> ;
                                                       <http://www.w3.org/2003/11/swrl#classPredicate> :BTPSolutionArchitect ;
                                                       <http://www.w3.org/2003/11/swrl#argument1> :x
                                                     ] ;
                                           rdf:rest rdf:nil
                                         ]
 ] .

[ <http://swrl.stanford.edu/ontologies/3.3/swrla.owl#isRuleEnabled> "true"^^xsd:boolean ;
   rdfs:comment "" ;
   rdfs:label "S2" ;
   rdf:type <http://www.w3.org/2003/11/swrl#Imp> ;
   <http://www.w3.org/2003/11/swrl#body> [ rdf:type <http://www.w3.org/2003/11/swrl#AtomList> ;
                                           rdf:first [ rdf:type <http://www.w3.org/2003/11/swrl#ClassAtom> ;
                                                       <http://www.w3.org/2003/11/swrl#classPredicate> :SAPEmployee ;
                                                       <http://www.w3.org/2003/11/swrl#argument1> :x
                                                     ] ;
                                           rdf:rest [ rdf:type <http://www.w3.org/2003/11/swrl#AtomList> ;
                                                      rdf:first [ rdf:type <http://www.w3.org/2003/11/swrl#IndividualPropertyAtom> ;
                                                                  <http://www.w3.org/2003/11/swrl#propertyPredicate> <http://xmlns.com/foaf/0.1/member> ;
                                                                  <http://www.w3.org/2003/11/swrl#argument1> :x ;
                                                                  <http://www.w3.org/2003/11/swrl#argument2> :SAPOrg2
                                                                ] ;
                                                      rdf:rest rdf:nil
                                                    ]
                                         ] ;
   <http://www.w3.org/2003/11/swrl#head> [ rdf:type <http://www.w3.org/2003/11/swrl#AtomList> ;
                                           rdf:first [ rdf:type <http://www.w3.org/2003/11/swrl#ClassAtom> ;
                                                       <http://www.w3.org/2003/11/swrl#classPredicate> :COILExpert ;
                                                       <http://www.w3.org/2003/11/swrl#argument1> :x
                                                     ] ;
                                           rdf:rest rdf:nil
                                         ]
 ] .

###  Generated by the OWL API (version 4.5.29.2024-05-13T12:11:03Z) https://github.com/owlcs/owlapi
